src/3d/prelude/EverParse3d.Prelude.fst
@@ -23,6 +23,8 @@ module LPLC = LowParse.Low.Combinators
 module U16 = FStar.UInt16
 module U32 = FStar.UInt32
 module U64 = FStar.UInt64
+open LowParse.Bytes
+module LS = EverParse3d.Serializer
 
 ////////////////////////////////////////////////////////////////////////////////
 // Parsers
@@ -314,3 +316,322 @@ inline_for_extraction noextract
 let read_unit
   : LPL.leaf_reader (parse_ret ())
   = LPLC.read_ret ()
+
+open Pulse.Lib.Core
+
+val serializes_to #nz #wk (#k:parser_kind nz wk) #t (p:parser k t) (x:t) (b:bytes) : prop
+let serializes_to p x b = LS.serializes_to p x b
+
+let in_codomain #nz #wk (#k:parser_kind nz wk) #t (p: parser k t) (x: t) = LS.in_codomain p x
+let codomain #nz #wk (#k:parser_kind nz wk) #t (p: parser k t) = LS.codomain p
+let serialize #nz #wk (#k:parser_kind nz wk) #t (p: parser k t) (x: codomain p) = LS.serialize p x
+
+let seqext1 #t (s1 s2 : Seq.seq t) :
+    Lemma (requires Seq.length s1 == 1 /\ Seq.length s2 == 1 /\ Seq.index s1 0 == Seq.index s2 0)
+      (ensures s1 == s2) =
+  Seq.cons_head_tail s1;
+  Seq.cons_head_tail s2;
+  Seq.lemma_empty (Seq.tail s1);
+  Seq.lemma_empty (Seq.tail s2)
+
+let seqlem #t (s1 : Seq.seq t) (x : t) :
+    Lemma (requires Seq.length s1 == 1)
+      (ensures Seq.upd s1 0 x == Seq.create 1 x) =
+  seqext1 (Seq.upd s1 0 x) (Seq.create 1 x)
+
+noeq type bv_api (t:Type0) : Type0 = {
+  v : t -> GTot nat;
+  shift8 : i:t -> o:t { v o == v i / 256 };
+  lsbyte : i:t -> o:UInt8.t { U8.v o == v i % 256 };
+}
+
+inline_for_extraction noextract let u8_api : bv_api U8.t = { v = U8.v; shift8 = (fun x -> U8.uint_to_t (U8.v x / 256)); lsbyte = (fun x -> U8.uint_to_t (U8.v x % 256)) }
+inline_for_extraction noextract let u16_api : bv_api U16.t = { v = U16.v; shift8 = (fun x -> U16.uint_to_t (U16.v x / 256)); lsbyte = (fun x -> U8.uint_to_t (U16.v x % 256)) }
+inline_for_extraction noextract let u32_api : bv_api U32.t = { v = U32.v; shift8 = (fun x -> U32.uint_to_t (U32.v x / 256)); lsbyte = (fun x -> U8.uint_to_t (U32.v x % 256)) }
+inline_for_extraction noextract let u64_api : bv_api U64.t = { v = U64.v; shift8 = (fun x -> U64.uint_to_t (U64.v x / 256)); lsbyte = (fun x -> U8.uint_to_t (U64.v x % 256)) }
+
+let pow2_8_mul (n:nat) : Lemma (pow2 (8 `op_Multiply` (n+1)) == 256 `op_Multiply` pow2 (8 `op_Multiply` n)) =
+  let k = op_Multiply 8 n in
+  Math.Lemmas.pow2_double_mult k;
+  Math.Lemmas.pow2_double_mult (k+1);
+  Math.Lemmas.pow2_double_mult (k+2);
+  Math.Lemmas.pow2_double_mult (k+3);
+  Math.Lemmas.pow2_double_mult (k+4);
+  Math.Lemmas.pow2_double_mult (k+5);
+  Math.Lemmas.pow2_double_mult (k+6);
+  Math.Lemmas.pow2_double_mult (k+7)
+
+let write_le_lem #t (n:pos) (api: bv_api t) (x:t { api.v x < Prims.pow2 (op_Multiply 8 n) }) :
+    Lemma (Seq.cons (api.lsbyte x) (pow2_8_mul (n-1); Endianness.n_to_le (n - 1) (api.v (api.shift8 x))) == Endianness.n_to_le n (api.v x)) =
+  pow2_8_mul (n-1);
+  let b1 = Seq.cons (api.lsbyte x) (Endianness.n_to_le (n - 1) (api.v (api.shift8 x))) in
+  let b2 = Endianness.n_to_le n (api.v x) in
+  Endianness.reveal_le_to_n b1;
+  Endianness.reveal_le_to_n b2;
+  Endianness.le_to_n_inj b1 b2
+
+noextract inline_for_extraction
+```pulse
+fn rec write_le #t (n:nat) (api: bv_api t) (x:t { api.v x < Prims.pow2 (op_Multiply 8 n) })
+    (arr: PA.array U8.t {SZ.fits (PA.length arr)})
+    (i: SZ.t { SZ.v i + n <= PA.length arr })
+  requires (exists* buf. PA.pts_to_range arr (SZ.v i) (PA.length arr) buf) ** emp
+  returns j:SZ.t
+  ensures
+    pure (SZ.v j == SZ.v i + n)
+    ** PA.pts_to_range arr (SZ.v i) (SZ.v j) (Endianness.n_to_le n (api.v x))
+    ** (exists* buf. PA.pts_to_range arr (SZ.v j) (PA.length arr) buf)
+    ** emp
+{
+  if (n = 0) {
+    with buf. assert (PA.pts_to_range arr (SZ.v i) (PA.length arr) buf);
+    PA.pts_to_range_split arr (SZ.v i) (SZ.v i) (PA.length arr);
+    FStar.Seq.Properties.slice_is_empty buf 0;
+    FStar.Seq.Properties.slice_length buf;
+    Seq.lemma_empty (Endianness.n_to_le 0 (api.v x));
+    i
+  } else {
+    PA.pts_to_range_split arr (SZ.v i) (SZ.v i + 1) (PA.length arr);
+    with buf1. assert PA.pts_to_range arr (SZ.v i) (SZ.v i + 1) buf1;
+    PA.pts_to_range_upd arr i (api.lsbyte x) #(SZ.v i);
+    seqlem buf1 (api.lsbyte x);
+    pow2_8_mul (n-1);
+    let j = write_le (n-1) api (api.shift8 x) arr (SZ.uint_to_t (SZ.v i + 1));
+    PA.pts_to_range_join arr (SZ.v i) (SZ.v i + 1) (SZ.v j);
+    write_le_lem n api x;
+    j
+  }
+}
+```
+
+let write_be_lem #t (n:pos) (api: bv_api t) (x:t { api.v x < Prims.pow2 (op_Multiply 8 n) }) :
+    Lemma (Seq.snoc (pow2_8_mul (n-1); Endianness.n_to_be (n - 1) (api.v (api.shift8 x))) (api.lsbyte x) == Endianness.n_to_be n (api.v x)) =
+  pow2_8_mul (n-1);
+  let b1 = Seq.snoc (Endianness.n_to_be (n - 1) (api.v (api.shift8 x))) (api.lsbyte x) in
+  let b2 = Endianness.n_to_be n (api.v x) in
+  Endianness.reveal_be_to_n b1;
+  Endianness.reveal_be_to_n b2;
+  Endianness.be_to_n_inj b1 b2
+
+noextract inline_for_extraction
+```pulse
+fn rec write_be #t (n:nat) (api: bv_api t) (x:t { api.v x < Prims.pow2 (op_Multiply 8 n) })
+    (arr: PA.array U8.t {SZ.fits (PA.length arr)})
+    (i: SZ.t { SZ.v i + n <= PA.length arr })
+  requires (exists* buf. PA.pts_to_range arr (SZ.v i) (PA.length arr) buf) ** emp
+  returns j:SZ.t
+  ensures
+    pure (SZ.v j == SZ.v i + n)
+    ** PA.pts_to_range arr (SZ.v i) (SZ.v j) (Endianness.n_to_be n (api.v x))
+    ** (exists* buf. PA.pts_to_range arr (SZ.v j) (PA.length arr) buf)
+    ** emp
+{
+  if (n = 0) {
+    with buf. assert (PA.pts_to_range arr (SZ.v i) (PA.length arr) buf);
+    PA.pts_to_range_split arr (SZ.v i) (SZ.v i) (PA.length arr);
+    FStar.Seq.Properties.slice_is_empty buf 0;
+    FStar.Seq.Properties.slice_length buf;
+    Seq.lemma_empty (Endianness.n_to_be 0 (api.v x));
+    i
+  } else {
+    pow2_8_mul (n-1);
+    let j = write_be (n-1) api (api.shift8 x) arr i;
+    PA.pts_to_range_split arr (SZ.v j) (SZ.v j + 1) (PA.length arr);
+    with buf1. assert PA.pts_to_range arr (SZ.v j) (SZ.v j + 1) buf1;
+    PA.pts_to_range_upd arr j (api.lsbyte x) #(SZ.v j);
+    seqlem buf1 (api.lsbyte x);
+    PA.pts_to_range_join arr (SZ.v i) (SZ.v j) (SZ.v j + 1);
+    write_be_lem n api x;
+    SZ.uint_to_t (SZ.v j + 1)
+  }
+}
+```
+
+let vprop_equiv_rfl #v0 #v1 (_:squash(v0==v1)) : vprop_equiv v0 v1 = vprop_equiv_refl v0
+
+let vprop_equiv_cng #p1 #p2 #p3 #p4 :
+    vprop_equiv p1 p3 -> vprop_equiv p2 p4 -> vprop_equiv (p1 ** p2) (p3 ** p4) =
+  vprop_equiv_cong _ _ _ _
+
+let pure_cng (#p #q:prop) (_:squash (p <==> q)) : vprop_equiv (pure p) (pure q) =
+  PropositionalExtensionality.apply p q;
+  vprop_equiv_refl (pure p)
+
+noextract [@@noextract_to "krml"] inline_for_extraction
+```pulse
+fn sub_stt' (#t:Type0) #pre #post pre' (post': t -> vprop) (hpre : vprop_equiv pre pre') (hpost: vprop_post_equiv post post') (k : unit -> stt t pre (fun x -> post x))
+  requires pre'
+  returns x:t
+  ensures post' x
+{
+  elim_vprop_equiv hpre;
+  rewrite pre' as pre;
+  let x:t = k ();
+  elim_vprop_equiv (elim_vprop_post_equiv _ _ hpost x);
+  rewrite post x as post' x;
+  x
+}
+```
+
+noextract [@@noextract_to "krml"] inline_for_extraction
+let sub_stt (#t:Type0) #pre #post pre' (post': t -> vprop) (hpre : vprop_equiv pre pre') (hpost: vprop_post_equiv post post') (k : stt t pre (fun x -> post x)) =
+  sub_stt' _ _ hpre hpost (fun _ -> k)
+
+noextract [@@noextract_to "krml"] inline_for_extraction
+let pulse_ser_be #nz #wk #k #t (p: parser #nz #wk k t) (api: bv_api t) n (x: t { api.v x < pow2 (8 `op_Multiply` n) /\ serializes_to p x (Endianness.n_to_be n (api.v x)) }) : pulse_ser_t p x emp =
+  fun arr i ->
+    sub_stt _ _ (vprop_equiv_rfl ()) (intro_vprop_post_equiv _ _ (fun x -> vprop_equiv_cng (vprop_equiv_cng (vprop_equiv_cng (pure_cng ()) (vprop_equiv_rfl ())) (vprop_equiv_rfl ())) (vprop_equiv_rfl ())))
+    (write_be n api x arr i)
+
+noextract [@@noextract_to "krml"] inline_for_extraction
+let pulse_ser_le #nz #wk #k #t (p: parser #nz #wk k t) (api: bv_api t) n (x: t { api.v x < pow2 (8 `op_Multiply` n) /\ serializes_to p x (Endianness.n_to_le n (api.v x)) }) : pulse_ser_t p x emp =
+  fun arr i ->
+    sub_stt _ _ (vprop_equiv_rfl ()) (intro_vprop_post_equiv _ _ (fun x -> vprop_equiv_cng (vprop_equiv_cng (vprop_equiv_cng (pure_cng ()) (vprop_equiv_rfl ())) (vprop_equiv_rfl ())) (vprop_equiv_rfl ())))
+    (write_le n api x arr i)
+
+let pulse_ser_u8 (x: U8.t) = LS.serializes_to_u8 x; pulse_ser_be parse____UINT8 u8_api 1 x
+let pulse_ser_u8be = pulse_ser_u8
+let pulse_ser_u16be (x: U16.t) = LS.serializes_to_u16be x; pulse_ser_be parse____UINT16BE u16_api 2 x
+let pulse_ser_u32be (x: U32.t) = LS.serializes_to_u32be x; pulse_ser_be parse____UINT32BE u32_api 4 x
+let pulse_ser_u64be (x: U64.t) = LS.serializes_to_u64be x; pulse_ser_be parse____UINT64BE u64_api 8 x
+let pulse_ser_u16le (x: U16.t) = LS.serializes_to_u16le x; pulse_ser_le parse____UINT16 u16_api 2 x
+let pulse_ser_u32le (x: U32.t) = LS.serializes_to_u32le x; pulse_ser_le parse____UINT32 u32_api 4 x
+let pulse_ser_u64le (x: U64.t) = LS.serializes_to_u64le x; pulse_ser_le parse____UINT64 u64_api 8 x
+
+noextract inline_for_extraction
+```pulse
+fn pulse_ser_dep_pair'
+    #nz1 (#k1:parser_kind nz1 WeakKindStrongPrefix) (#t1: Type0) (p1: parser k1 t1)
+    #nz2 #wk2 (#k2:parser_kind nz2 wk2) (#t2: t1 -> Type0) (p2: (x: t1) -> parser k2 (t2 x))
+    (x1: erased t1) (x2: erased (t2 x1))
+    (frame: vprop)
+    (s1: pulse_ser_t p1 (reveal x1) frame)
+    (s2: pulse_ser_t (p2 x1) (reveal x2) frame)
+    (arr: PA.array FStar.UInt8.t {SZ.fits (PA.length arr)})
+    (i: SZ.t { SZ.v i <= PA.length arr /\ serialized_fits (parse_dep_pair p1 p2) (| reveal x1, reveal x2 |) (PA.length arr - SZ.v i) })
+  requires (exists* buf. PA.pts_to_range arr (SZ.v i) (PA.length arr) buf) ** frame
+  returns j:SZ.t
+  ensures
+    pure (SZ.v j == SZ.v i + Seq.length (serialize (parse_dep_pair p1 p2) (reveal (hide (| reveal x1, reveal x2 |)))))
+    ** PA.pts_to_range arr (SZ.v i) (SZ.v j) (serialize (parse_dep_pair p1 p2) (reveal (hide (| reveal x1, reveal x2 |))))
+    ** (exists* buf. PA.pts_to_range arr (SZ.v j) (PA.length arr) buf)
+    ** frame
+{
+  LS.in_codomain_dtuple2 p1 p2 x1 x2;
+  LS.serializes_to_dtuple2 p1 p2 x1 x2;
+  let k = s1 arr i;
+  let j = s2 arr k;
+  PA.pts_to_range_join arr (SZ.v i) (SZ.v k) (SZ.v j);
+  j
+}
+```
+
+inline_for_extraction noextract
+let pulse_ser_dep_pair
+    #nz1 (#k1:parser_kind nz1 WeakKindStrongPrefix) (#t1: Type0) (p1: parser k1 t1)
+    #nz2 #wk2 (#k2:parser_kind nz2 wk2) (#t2: t1 -> Type0) (p2: (x: t1) -> parser k2 (t2 x))
+    (x1: erased t1) (x2: erased (t2 x1))
+    (frame: vprop)
+    (s1: pulse_ser_t p1 x1 frame)
+    (s2: pulse_ser_t (p2 x1) x2 frame) :
+    pulse_ser_t (parse_dep_pair p1 p2) (| reveal x1, reveal x2 |) frame =
+  fun arr i ->
+    sub_stt _ _ (vprop_equiv_rfl ()) (intro_vprop_post_equiv _ _ (fun x -> vprop_equiv_cng (vprop_equiv_cng (vprop_equiv_cng (pure_cng ()) (vprop_equiv_rfl ())) (vprop_equiv_rfl ())) (vprop_equiv_rfl ())))
+    (pulse_ser_dep_pair' p1 p2 x1 x2 frame s1 s2 arr i)
+
+inline_for_extraction noextract
+```pulse
+fn pulse_ser_pair'
+    #nz1 (#k1:parser_kind nz1 WeakKindStrongPrefix) (#t1: Type0) (p1: parser k1 t1)
+    #nz2 #wk2 (#k2:parser_kind nz2 wk2) (#t2: Type0) (p2: parser k2 t2)
+    (x1: erased t1) (x2: erased t2)
+    (frame: vprop)
+    (s1: pulse_ser_t p1 (reveal x1) frame)
+    (s2: pulse_ser_t p2 (reveal x2) frame)
+    (arr: PA.array FStar.UInt8.t {SZ.fits (PA.length arr)})
+    (i: SZ.t { SZ.v i <= PA.length arr /\ serialized_fits (parse_pair p1 p2) (reveal x1, reveal x2) (PA.length arr - SZ.v i) })
+  requires (exists* buf. PA.pts_to_range arr (SZ.v i) (PA.length arr) buf) ** frame
+  returns j:SZ.t
+  ensures
+    pure (SZ.v j == SZ.v i + Seq.length (serialize (parse_pair p1 p2) (reveal (hide (reveal x1, reveal x2)))))
+    ** PA.pts_to_range arr (SZ.v i) (SZ.v j) (serialize (parse_pair p1 p2) (reveal (hide (reveal x1, reveal x2))))
+    ** (exists* buf. PA.pts_to_range arr (SZ.v j) (PA.length arr) buf)
+    ** frame
+{
+  LS.in_codomain_nondep_then p1 p2 x1 x2;
+  LS.serializes_to_nondep_then p1 p2 x1 x2;
+  let k = s1 arr i;
+  let j = s2 arr k;
+  PA.pts_to_range_join arr (SZ.v i) (SZ.v k) (SZ.v j);
+  j
+}
+```
+
+inline_for_extraction noextract
+let pulse_ser_pair
+    #nz1 (#k1:parser_kind nz1 WeakKindStrongPrefix) (#t1: Type0) (p1: parser k1 t1)
+    #nz2 #wk2 (#k2:parser_kind nz2 wk2) (#t2: Type0) (p2: parser k2 t2)
+    (x1: erased t1) (x2: erased t2)
+    (frame: vprop)
+    (s1: pulse_ser_t p1 x1 frame)
+    (s2: pulse_ser_t p2 x2 frame) :
+    pulse_ser_t (parse_pair p1 p2) (reveal x1, reveal x2) frame =
+  fun arr i ->
+    sub_stt _ _ (vprop_equiv_rfl ()) (intro_vprop_post_equiv _ _ (fun x -> vprop_equiv_cng (vprop_equiv_cng (vprop_equiv_cng (pure_cng ()) (vprop_equiv_rfl ())) (vprop_equiv_rfl ())) (vprop_equiv_rfl ())))
+    (pulse_ser_pair' p1 p2 x1 x2 frame s1 s2 arr i)
+
+inline_for_extraction noextract
+```pulse
+fn pulse_ser_ret' (#t:Type0) (v:t)
+    (arr: PA.array FStar.UInt8.t {SZ.fits (PA.length arr)})
+    (i: SZ.t { SZ.v i <= PA.length arr /\ serialized_fits (parse_ret v) v (PA.length arr - SZ.v i) })
+  requires (exists* buf. PA.pts_to_range arr (SZ.v i) (PA.length arr) buf) ** emp
+  returns j:SZ.t
+  ensures
+    pure (SZ.v j == SZ.v i + Seq.length (serialize (parse_ret v) v))
+    ** PA.pts_to_range arr (SZ.v i) (SZ.v j) (serialize (parse_ret v) v)
+    ** (exists* buf. PA.pts_to_range arr (SZ.v j) (PA.length arr) buf)
+    ** emp
+{
+  with buf. assert (PA.pts_to_range arr (SZ.v i) (PA.length arr) buf);
+  PA.pts_to_range_split arr (SZ.v i) (SZ.v i) (PA.length arr);
+  Seq.Properties.slice_is_empty buf 0;
+  Seq.Properties.slice_length buf;
+  LS.serializes_to_ret v;
+  assert pure (Seq.length (Seq.empty #U8.t) == 0);
+  i
+}
+
+```
+inline_for_extraction noextract
+let pulse_ser_ret (#t:Type0) (v:t) : pulse_ser_t (parse_ret v) v emp =
+  fun arr i ->
+  sub_stt _ _ (vprop_equiv_rfl ()) (intro_vprop_post_equiv _ _ (fun _ -> vprop_equiv_cng (vprop_equiv_cng (vprop_equiv_cng (pure_cng ()) (vprop_equiv_rfl ())) (vprop_equiv_rfl ())) (vprop_equiv_rfl ())))
+  (pulse_ser_ret' v arr i)
+
+let pulse_size_t #nz #wk #k #t (p: parser #nz #wk k t) (x: erased (codomain p)) (frame: vprop) =
+  stt SZ.t frame (fun j -> frame ** pure (serialized_fits p x (SZ.v j)))
+
+noextract inline_for_extraction
+```pulse
+fn pulse_size_fixed' #nz #wk #k (#t:Type0) (p: parser #nz #wk k t) (x: erased (codomain p)) (sz: SZ.t {serialized_fits p x (SZ.v sz)})
+  requires emp
+  returns j:SZ.t
+  ensures emp ** pure (serialized_fits p x (SZ.v j))
+{
+  sz
+}
+```
+
+noextract inline_for_extraction
+let pulse_size_fixed #nz #wk #k #t (p: parser #nz #wk k t) (x: erased (codomain p)) (sz: SZ.t {serialized_fits p x (SZ.v sz)}) :
+    pulse_size_t p x emp =
+  pulse_size_fixed' p x sz
+
+inline_for_extraction let pulse_size_u8 (x: U8.t) = LS.serializes_to_u8 x; pulse_size_fixed parse____UINT8 x (SZ.uint_to_t 1)
+inline_for_extraction let pulse_size_u16be (x: U16.t) = LS.serializes_to_u16be x; pulse_size_fixed parse____UINT16BE x (SZ.uint_to_t 2)
+inline_for_extraction let pulse_size_u32be (x: U32.t) = LS.serializes_to_u32be x; pulse_size_fixed parse____UINT32BE x (SZ.uint_to_t 4)
+inline_for_extraction let pulse_size_u64be (x: U64.t) = LS.serializes_to_u64be x; pulse_size_fixed parse____UINT64BE x (SZ.uint_to_t 8)
+inline_for_extraction let pulse_size_u16le (x: U16.t) = LS.serializes_to_u16le x; pulse_size_fixed parse____UINT16 x (SZ.uint_to_t 2)
+inline_for_extraction let pulse_size_u32le (x: U32.t) = LS.serializes_to_u32le x; pulse_size_fixed parse____UINT32 x (SZ.uint_to_t 4)
+inline_for_extraction let pulse_size_u64le (x: U64.t) = LS.serializes_to_u64le x; pulse_size_fixed parse____UINT64 x (SZ.uint_to_t 8)
