src/3d/prelude/EverParse3d.Serializer.fst
@@ -1,0 +1,125 @@
+module EverParse3d.Serializer
+open LowParse.Bytes
+open LowParse.Spec.Base
+open LowParse.Spec.Combinators
+
+let in_codomain p x = exists y. p y == Some (x, Seq.length y)
+
+let serialize p x = FStar.IndefiniteDescription.indefinite_description_ghost bytes (fun y -> p y == Some (x, Seq.length y))
+
+let serializes_to_intro p x b = LowParse.Spec.Base.parse_injective p (serialize p x) b
+
+let serialize_inj p x1 x2 = serializes_to_intro p x1 (serialize p x2)
+
+let serializes_to_ret v = serializes_to_intro (parse_ret v) v Seq.empty
+
+let serializes_to_filter p f x =
+  parse_filter_eq p f (serialize p x);
+  serializes_to_intro (parse_filter p f) x (serialize p x)
+
+let in_codomain_filter p f x =
+  introduce in_codomain (parse_filter p f) x ==> in_codomain p x with _.
+    parse_filter_eq p f (serialize (parse_filter p f) x);
+  introduce in_codomain p x ==> in_codomain (parse_filter p f) x with _. serializes_to_filter p f x
+
+let serializes_to_dtuple2 p1 p2 x1 x2 =
+  let b1 = serialize p1 x1 in
+  let b2 = serialize (p2 x1) x2 in
+  LowParse.Spec.Base.parse_strong_prefix p1 b1 (Seq.append b1 b2);
+  LowParse.Spec.Combinators.parse_dtuple2_eq p1 p2 (Seq.append b1 b2);
+  FStar.Seq.Properties.append_slices b1 b2;
+  serializes_to_intro (parse_dtuple2 p1 p2) (| x1, x2 |) (Seq.append b1 b2)
+
+let in_codomain_dtuple2 p1 p2 x1 x2 =
+  introduce in_codomain p1 x1 /\ in_codomain (p2 x1) x2 ==> in_codomain (parse_dtuple2 p1 p2) (| x1, x2 |) with _. serializes_to_dtuple2 p1 p2 x1 x2;
+  introduce in_codomain (parse_dtuple2 p1 p2) (|x1, x2|) ==> in_codomain p1 x1 /\ in_codomain (p2 x1) x2 with _. begin
+    let b = serialize (parse_dtuple2 p1 p2) (| x1, x2 |) in
+    LowParse.Spec.Combinators.parse_dtuple2_eq p1 p2 b;
+    let Some (x1', c1) = p1 b in
+    let b1 = Seq.slice b 0 c1 in
+    LowParse.Spec.Base.parse_strong_prefix p1 b b1;
+    serializes_to_intro p1 x1 b1
+  end
+
+let serializes_to_nondep_then p1 p2 x1 x2 =
+  let b1 = serialize p1 x1 in
+  let b2 = serialize p2 x2 in
+  LowParse.Spec.Base.parse_strong_prefix p1 b1 (Seq.append b1 b2);
+  LowParse.Spec.Combinators.nondep_then_eq p1 p2 (Seq.append b1 b2);
+  FStar.Seq.Properties.append_slices b1 b2;
+  serializes_to_intro (nondep_then p1 p2) (x1, x2) (Seq.append b1 b2)
+
+let in_codomain_nondep_then p1 p2 x1 x2 =
+  introduce in_codomain p1 x1 /\ in_codomain p2 x2 ==> in_codomain (nondep_then p1 p2) (x1, x2) with _. serializes_to_nondep_then p1 p2 x1 x2;
+  introduce in_codomain (nondep_then p1 p2) (x1, x2) ==> in_codomain p1 x1 /\ in_codomain p2 x2 with _. begin
+    let b = serialize (nondep_then p1 p2) (x1, x2) in
+    LowParse.Spec.Combinators.nondep_then_eq p1 p2 b;
+    let Some (x1', c1) = p1 b in
+    let b1 = Seq.slice b 0 c1 in
+    LowParse.Spec.Base.parse_strong_prefix p1 b b1;
+    serializes_to_intro p1 x1 b1
+  end
+
+let serializes_to_u8 x =
+  LowParse.Spec.Int.parse_u8_spec (Endianness.n_to_be 1 (UInt8.v x));
+  serializes_to_intro LowParse.Spec.Int.parse_u8 x (Endianness.n_to_be 1 (UInt8.v x))
+
+let serializes_to_u16be x =
+  LowParse.Spec.Int.parse_u16_spec (Endianness.n_to_be 2 (UInt16.v x));
+  serializes_to_intro LowParse.Spec.Int.parse_u16 x (Endianness.n_to_be 2 (UInt16.v x))
+
+let serializes_to_u32be x =
+  LowParse.Spec.Int.parse_u32_spec (Endianness.n_to_be 4 (UInt32.v x));
+  serializes_to_intro LowParse.Spec.Int.parse_u32 x (Endianness.n_to_be 4 (UInt32.v x))
+
+let serializes_to_u64be x =
+  LowParse.Spec.Int.parse_u64_spec (Endianness.n_to_be 8 (UInt64.v x));
+  serializes_to_intro LowParse.Spec.Int.parse_u64 x (Endianness.n_to_be 8 (UInt64.v x))
+
+let serializes_to_u16le x =
+  LowParse.Spec.BoundedInt.parse_u16_le_spec (Endianness.n_to_le 2 (UInt16.v x));
+  serializes_to_intro LowParse.Spec.BoundedInt.parse_u16_le x (Endianness.n_to_le 2 (UInt16.v x))
+
+let serializes_to_u32le x =
+  LowParse.Spec.BoundedInt.parse_u32_le_spec (Endianness.n_to_le 4 (UInt32.v x));
+  serializes_to_intro LowParse.Spec.BoundedInt.parse_u32_le x (Endianness.n_to_le 4 (UInt32.v x))
+
+let serializes_to_u64le x =
+  LowParse.Spec.Int.parse_u64_le_spec (Endianness.n_to_le 8 (UInt64.v x));
+  serializes_to_intro LowParse.Spec.Int.parse_u64_le x (Endianness.n_to_le 8 (UInt64.v x))
+
+let serializes_to_fldata p sz x =
+  serializes_to_intro (parse_fldata p sz) x (serialize p x)
+
+let in_codomain_fldata p sz x =
+  introduce in_codomain (parse_fldata p sz) x ==> in_codomain p x /\ Seq.length (serialize p x) == sz with _.
+    serializes_to_intro p x (serialize (parse_fldata p sz) x);
+  introduce in_codomain p x /\ Seq.length (serialize p x) == sz ==> in_codomain (parse_fldata p sz) x with _.
+    serializes_to_fldata p sz x
+
+let serializes_to_list_nil p =
+  parse_list_eq p Seq.empty;
+  serializes_to_intro (parse_list p) [] Seq.empty
+
+let serializes_to_list_cons p x xs =
+  let b1 = serialize p x in
+  let b2 = serialize (parse_list p) xs in
+  let bs = Seq.append b1 b2 in
+  LowParse.Spec.Base.parse_strong_prefix p b1 bs;
+  parse_list_eq p bs;
+  Seq.append_slices b1 b2;
+  serializes_to_intro (parse_list p) (x::xs) bs
+
+let in_codomain_list_cons p x xs =
+  introduce in_codomain (parse_list p) (x::xs) ==>
+      in_codomain p x /\ Seq.length (serialize p x) > 0 /\ in_codomain (parse_list p) xs with _.
+  begin
+    let bs = serialize (parse_list p) (x::xs) in
+    parse_list_eq p bs;
+    let Some (x', n) = p bs in
+    LowParse.Spec.Base.parse_strong_prefix p bs (Seq.slice bs 0 n);
+    serializes_to_intro p x (Seq.slice bs 0 n)
+  end;
+  introduce in_codomain p x /\ Seq.length (serialize p x) > 0 /\ in_codomain (parse_list p) xs ==>
+      in_codomain (parse_list p) (x::xs) with _.
+    serializes_to_list_cons p x xs
